Further forward progress on proofs
Start removing unfold from places where I have no good reason per Nik's advice
Start favoring #set-options and #push-options/#pop-options

qtesla/code/Hacl.Impl.QTesla.Globals.fst
@@ -22,36 +22,19 @@ module B = LowStar.Buffer
 
 #reset-options "--z3rlimit 100 --max_fuel 1 --max_ifuel 1"
 
-//let is_elem (e:elem_base) = let x = elem_v e in let q = elem_v params_q in -q < x /\ x < q
-
 let is_elem_int (e:int) : GTot bool =
   let q = elem_v params_q in
   -q < e && e < q
-
-(*assume IntTypeInequality : ~(I32.t == I64.t) /\ ~(I32.t == int) /\ ~(I64.t == int) 
-
-let is_elem (#a:Type) (e:a) =
-  let q = elem_v params_q in
-  (a == I64.t \/ a == I32.t \/ a == int) /\
-  ((a == I32.t) ==> (let x = I32.v e in is_elem_int x)) /\
-  ((a == I64.t) ==> (let x = I64.v e in is_elem_int x)) /\
-  ((a == int) ==> (is_elem_int e))*)
 
 let is_elem (e:elem_base) : GTot bool = let x = elem_v e in is_elem_int x
 let is_elem_i32 (e:I32.t) : GTot bool = let x = I32.v e in is_elem_int x
 let is_elem_i64 (e:I64.t) : GTot bool = let x = I64.v e in is_elem_int x
 
-//let test _ = let e:I32.t = 0l in assert(is_elem e)
-
-//#reset-options "--z3rlimit 100 --max_fuel 0 --max_ifuel 0"
-
 type elem = elem_base
 let is_uelem e = let x = uelem_v e in let q = elem_v params_q in 0 <= x /\ x < q
 type uelem = uelem_base
 type poly = lbuffer elem params_n
-type poly_pred pred = lbuffer (e:elem{pred e}) params_n
-type poly_k = lbuffer elem (params_k *. params_n)
-type poly_k_pred pred = lbuffer (e:elem{pred e}) (params_k *. params_n)
+type poly_k = lbuffer elem (params_k *! params_n)
 
 let is_montgomery (e:elem) = 0 <= elem_v e /\ elem_v e < 2 * elem_v params_q
 let is_corrected (e:elem) = -(elem_v params_q / 2) < elem_v e /\ elem_v e <= elem_v params_q / 2
@@ -64,63 +47,57 @@ let is_z_accepted (e:elem) = let b = elem_v params_B in let s = elem_v params_U 
 let is_sparse_mul_output (e:elem) = (-65536) <= elem_v e /\ elem_v e <= 65536 // [-2^16, 2^16]; see sparse_mul for comments
 let is_sparse_mul32_output (e:elem) = let q = elem_v params_q in -q <= elem_v e /\ elem_v e < 2 * q
 
-(*{:pattern (bget h p i)}*)
-//let is_poly_pred (h:HS.mem) (p:poly) (pred:(elem -> Type0)) (k:nat{k <= v params_k * v params_n}) = forall i . (i < k) ==> (pred (bget h p i))
+let is_poly_montgomery_i (h:HS.mem) (p:poly) (j:nat{j <= v params_n}) = forall (i:nat{i < j}). {:pattern is_montgomery (bget h p i)} is_montgomery (bget h p i)
+let is_poly_corrected_i (h:HS.mem) (p:poly) (j:nat{j <= v params_n}) = forall (i:nat{i < j}). {:pattern is_corrected (bget h p i)}  is_corrected (bget h p i)
+let is_poly_sampler_output_i (h:HS.mem) (p:poly) (j:nat{j <= v params_n}) = forall (i:nat{i < j}). {:pattern is_sampler_output (bget h p i)} is_sampler_output (bget h p i)
+let is_poly_y_sampler_output_i (h:HS.mem) (p:poly) (j:nat{j <= v params_n}) = forall (i:nat{i < j}). {:pattern is_y_sampler_output (bget h p i)} is_y_sampler_output (bget h p i)
+let is_poly_pk_i (h:HS.mem) (p:poly) (j:nat{j <= v params_n}) = forall (i:nat{i < j}). {:pattern is_pk (bget h p i)} is_pk (bget h p i)
+let is_poly_sk_i (h:HS.mem) (p:poly) (j:nat{j <= v params_n}) = forall (i:nat{i < j}). {:pattern is_sk (bget h p i)} is_sk (bget h p i)
+let is_poly_pmq_i (h:HS.mem) (p:poly) (j:nat{j <= v params_n}) = forall (i:nat{i < j}). {:pattern is_pmq (bget h p i)} is_pmq (bget h p i)
+let is_poly_z_accepted_i (h:HS.mem) (p:poly) (j:nat{j <= v params_n}) = forall (i:nat{i < j}). {:pattern is_z_accepted (bget h p i)} is_z_accepted (bget h p i)
+let is_poly_sparse_mul_output_i (h:HS.mem) (p:poly) (j:nat{j <= v params_n}) = forall (i:nat{i < j}). {:pattern is_sparse_mul_output (bget h p i)} is_sparse_mul_output (bget h p i)
+let is_poly_sparse_mul32_output_i (h:HS.mem) (p:poly) (j:nat{j <= v params_n}) = forall (i:nat{i < j}). {:pattern is_sparse_mul32_output (bget h p i)} is_sparse_mul32_output (bget h p i)
 
-//let is_poly_montgomery_k (h:HS.mem) (p:poly) = is_poly_pred h p is_montgomery
-//let is_poly_corrected_k (h:HS.mem) (p:poly) = is_poly_pred h p is_corrected
-//let is_poly_sampler_output_k (h:HS.mem) (p:poly) = is_poly_pred h p is_sampler_output
+let is_poly_k_montgomery_i (h:HS.mem) (p:poly_k) (j:nat{j <= v params_k * v params_n}) = forall (i:nat{i < j}). {:pattern is_montgomery (bget h p i)} is_montgomery (bget h p i)
+let is_poly_k_corrected_i (h:HS.mem) (p:poly_k) (j:nat{j <= v params_k * v params_n}) = forall (i:nat{i < j}). {:pattern is_corrected (bget h p i)} is_corrected (bget h p i)
+let is_poly_k_sampler_output_i (h:HS.mem) (p:poly_k) (j:nat{j <= v params_k * v params_n}) = forall (i:nat{i < j}). {:pattern is_sampler_output (bget h p i)} is_sampler_output (bget h p i)
+let is_poly_k_pk_i (h:HS.mem) (p:poly_k) (j:nat{j <= v params_k * v params_n}) = forall (i:nat{i < j}). {:pattern is_pk (bget h p i)} is_pk (bget h p i)
+let is_poly_k_sk_i (h:HS.mem) (p:poly_k) (j:nat{j <= v params_k * v params_n}) = forall (i:nat{i < j}). {:pattern is_sk (bget h p i)} is_sk (bget h p i)
 
-unfold let is_poly_montgomery_i (h:HS.mem) (p:poly) (j:nat{j <= v params_n}) = forall (i:nat{i < j}). {:pattern is_montgomery (bget h p i)} is_montgomery (bget h p i)
-unfold let is_poly_corrected_i (h:HS.mem) (p:poly) (j:nat{j <= v params_n}) = forall (i:nat{i < j}). {:pattern is_corrected (bget h p i)}  is_corrected (bget h p i)
-unfold let is_poly_sampler_output_i (h:HS.mem) (p:poly) (j:nat{j <= v params_n}) = forall (i:nat{i < j}). {:pattern is_sampler_output (bget h p i)} is_sampler_output (bget h p i)
-unfold let is_poly_y_sampler_output_i (h:HS.mem) (p:poly) (j:nat{j <= v params_n}) = forall (i:nat{i < j}). {:pattern is_y_sampler_output (bget h p i)} is_y_sampler_output (bget h p i)
-unfold let is_poly_pk_i (h:HS.mem) (p:poly) (j:nat{j <= v params_n}) = forall (i:nat{i < j}). {:pattern is_pk (bget h p i)} is_pk (bget h p i)
-unfold let is_poly_sk_i (h:HS.mem) (p:poly) (j:nat{j <= v params_n}) = forall (i:nat{i < j}). {:pattern is_sk (bget h p i)} is_sk (bget h p i)
-unfold let is_poly_pmq_i (h:HS.mem) (p:poly) (j:nat{j <= v params_n}) = forall (i:nat{i < j}). {:pattern is_pmq (bget h p i)} is_pmq (bget h p i)
-unfold let is_poly_z_accepted_i (h:HS.mem) (p:poly) (j:nat{j <= v params_n}) = forall (i:nat{i < j}). {:pattern is_z_accepted (bget h p i)} is_z_accepted (bget h p i)
-unfold let is_poly_sparse_mul_output_i (h:HS.mem) (p:poly) (j:nat{j <= v params_n}) = forall (i:nat{i < j}). {:pattern is_sparse_mul_output (bget h p i)} is_sparse_mul_output (bget h p i)
-unfold let is_poly_sparse_mul32_output_i (h:HS.mem) (p:poly) (j:nat{j <= v params_n}) = forall (i:nat{i < j}). {:pattern is_sparse_mul32_output (bget h p i)} is_sparse_mul32_output (bget h p i)
+let is_poly_montgomery (h:HS.mem) (p:poly) = is_poly_montgomery_i h p (v params_n)
+let is_poly_corrected (h:HS.mem) (p:poly) = is_poly_corrected_i h p (v params_n)
+let is_poly_sampler_output (h:HS.mem) (p:poly) = is_poly_sampler_output_i h p (v params_n)
+let is_poly_y_sampler_output (h:HS.mem) (p:poly) = is_poly_y_sampler_output_i h p (v params_n)
+let is_poly_pk (h:HS.mem) (p:poly) = is_poly_pk_i h p (v params_n)
+let is_poly_sk (h:HS.mem) (p:poly) = is_poly_sk_i h p (v params_n)
+let is_poly_pmq (h:HS.mem) (p:poly) = is_poly_pmq_i h p (v params_n)
+let is_poly_z_accepted (h:HS.mem) (p:poly) = is_poly_z_accepted_i h p (v params_n)
+let is_poly_sparse_mul_output (h:HS.mem) (p:poly) = is_poly_sparse_mul_output_i h p (v params_n)
+let is_poly_sparse_mul32_output (h:HS.mem) (p:poly) = is_poly_sparse_mul32_output_i h p (v params_n)
 
-unfold let is_poly_k_montgomery_i (h:HS.mem) (p:poly_k) (j:nat{j <= v params_k * v params_n}) = forall (i:nat{i < j}). {:pattern is_montgomery (bget h p i)} is_montgomery (bget h p i)
-unfold let is_poly_k_corrected_i (h:HS.mem) (p:poly_k) (j:nat{j <= v params_k * v params_n}) = forall (i:nat{i < j}). {:pattern is_corrected (bget h p i)} is_corrected (bget h p i)
-unfold let is_poly_k_sampler_output_i (h:HS.mem) (p:poly_k) (j:nat{j <= v params_k * v params_n}) = forall (i:nat{i < j}). {:pattern is_sampler_output (bget h p i)} is_sampler_output (bget h p i)
-unfold let is_poly_k_pk_i (h:HS.mem) (p:poly_k) (j:nat{j <= v params_k * v params_n}) = forall (i:nat{i < j}). {:pattern is_pk (bget h p i)} is_pk (bget h p i)
-unfold let is_poly_k_sk_i (h:HS.mem) (p:poly_k) (j:nat{j <= v params_k * v params_n}) = forall (i:nat{i < j}). {:pattern is_sk (bget h p i)} is_sk (bget h p i)
+let is_poly_k_montgomery (h:HS.mem) (p:poly_k) = is_poly_k_montgomery_i h p (v params_k * v params_n)
+let is_poly_k_corrected (h:HS.mem) (p:poly_k) = is_poly_k_corrected_i h p (v params_k * v params_n)
+let is_poly_k_sampler_output (h:HS.mem) (p:poly_k) = is_poly_k_sampler_output_i h p (v params_k * v params_n)
+let is_poly_k_pk (h:HS.mem) (p:poly_k) = is_poly_k_pk_i h p (v params_k * v params_n)
+let is_poly_k_sk (h:HS.mem) (p:poly_k) = is_poly_k_sk_i h p (v params_k * v params_n)
 
-unfold let is_poly_montgomery (h:HS.mem) (p:poly) = is_poly_montgomery_i h p (v params_n)
-unfold let is_poly_corrected (h:HS.mem) (p:poly) = is_poly_corrected_i h p (v params_n)
-unfold let is_poly_sampler_output (h:HS.mem) (p:poly) = is_poly_sampler_output_i h p (v params_n)
-unfold let is_poly_y_sampler_output (h:HS.mem) (p:poly) = is_poly_y_sampler_output_i h p (v params_n)
-unfold let is_poly_pk (h:HS.mem) (p:poly) = is_poly_pk_i h p (v params_n)
-unfold let is_poly_sk (h:HS.mem) (p:poly) = is_poly_sk_i h p (v params_n)
-unfold let is_poly_pmq (h:HS.mem) (p:poly) = is_poly_pmq_i h p (v params_n)
-unfold let is_poly_z_accepted (h:HS.mem) (p:poly) = is_poly_z_accepted_i h p (v params_n)
-unfold let is_poly_sparse_mul_output (h:HS.mem) (p:poly) = is_poly_sparse_mul_output_i h p (v params_n)
-unfold let is_poly_sparse_mul32_output (h:HS.mem) (p:poly) = is_poly_sparse_mul32_output_i h p (v params_n)
-
-unfold let is_poly_k_montgomery (h:HS.mem) (p:poly_k) = is_poly_k_montgomery_i h p (v params_k * v params_n)
-unfold let is_poly_k_corrected (h:HS.mem) (p:poly_k) = is_poly_k_corrected_i h p (v params_k * v params_n)
-unfold let is_poly_k_sampler_output (h:HS.mem) (p:poly_k) = is_poly_k_sampler_output_i h p (v params_k * v params_n)
-unfold let is_poly_k_pk (h:HS.mem) (p:poly_k) = is_poly_k_pk_i h p (v params_k * v params_n)
-unfold let is_poly_k_sk (h:HS.mem) (p:poly_k) = is_poly_k_sk_i h p (v params_k * v params_n)
-
-unfold let is_poly_equal (h0 h1:HS.mem) (p:poly) = 
+let is_poly_equal (h0 h1:HS.mem) (p:poly) = 
     forall (i:nat{i < v params_n}) . {:pattern bget h1 p i} bget h0 p i == bget h1 p i
-unfold let is_poly_equal_except (h0 h1:HS.mem) (p:poly) (k:nat{k < v params_n}) = 
+let is_poly_equal_except (h0 h1:HS.mem) (p:poly) (k:nat{k < v params_n}) = 
     forall (i:nat{i < v params_n /\ i <> k}) . {:pattern bget h1 p i} bget h0 p i == bget h1 p i
-unfold let is_poly_k_equal (h0 h1:HS.mem) (p:poly_k) = 
+let is_poly_k_equal (h0 h1:HS.mem) (p:poly_k) = 
     forall (i:nat{i < v params_n * v params_k}) . {:pattern bget h1 p i} bget h0 p i == bget h1 p i
 
-unfold let is_sparse_elem_sk (e:sparse_elem) = -(pow2 (v params_s_bits)) <= sparse_v e /\ sparse_v e < pow2 (v params_s_bits)
-//let is_s_sk (h:HS.mem) (s:lbuffer sparse_elem params_n) =
-//    forall (i:nat{i < v params_n}) . {:pattern is_sparse_elem_sk (bget h s i)} is_sparse_elem_sk (bget h s i)
+let is_sparse_elem_sk (e:sparse_elem) = -(pow2 (v params_s_bits)) <= sparse_v e /\ sparse_v e < pow2 (v params_s_bits)
 let is_s_sk (h:HS.mem) (s:lbuffer sparse_elem params_n) =
-    forall (i:nat{i < v params_n}) . is_sparse_elem_sk (bget h s i)
-//let is_e_sk (h:HS.mem) (e:lbuffer sparse_elem (params_n *. params_k)) =
-//    forall (i:nat{i < v params_n * v params_k}) . {:pattern is_sparse_elem_sk (bget h e i)} is_sparse_elem_sk (bget h e i)
-let is_e_sk (h:HS.mem) (e:lbuffer sparse_elem (params_n *. params_k)) =
-    forall (i:nat{i < v params_n * v params_k}) . is_sparse_elem_sk (bget h e i)
+    forall (i:nat{i < v params_n}) . {:pattern is_sparse_elem_sk (bget h s i)} is_sparse_elem_sk (bget h s i)
+let is_s_equal (h0 h1:HS.mem) (s:lbuffer sparse_elem params_n) =
+    forall (i:nat{i < v params_n}) . {:pattern bget h1 s i} bget h0 s i == bget h1 s i
+let is_e_sk (h:HS.mem) (e:lbuffer sparse_elem (params_n *! params_k)) =
+    forall (i:nat{i < v params_n * v params_k}) . {:pattern is_sparse_elem_sk (bget h e i)} is_sparse_elem_sk (bget h e i)
+let is_e_equal (h0 h1:HS.mem) (e:lbuffer sparse_elem (params_n *! params_k)) =
+    forall (i:nat{i < v params_n}) . {:pattern bget h1 e i} bget h0 e i == bget h1 e i
+
 
 (*let frame_is_poly_sampler_output_i (h0 h1: HS.mem) (p: poly) (i:nat{i <= v params_n}) (l:B.loc) : Lemma
     (requires is_poly_sampler_output_i h0 p i /\ modifies l h0 h1 /\ disjoint l (gsub p (size 0) (size i)))
@@ -155,17 +132,17 @@ val poly_k_create:
     (requires fun _ -> True)
     (ensures fun h0 r h1 -> live h1 r /\ stack_allocated r h0 h1 (Seq.create (v params_n * v params_k) (to_elem 0)))
 
-let poly_k_create _ = create (params_n *. params_k) (to_elem 0)
+let poly_k_create _ = create (params_n *! params_k) (to_elem 0)
 
-unfold val get_poly: p: poly_k -> k: size_t{k <. params_k} -> GTot poly
-let get_poly p k = gsub p (k *. params_n) params_n
+val get_poly: p: poly_k -> k: size_t{k <. params_k} -> GTot poly
+let get_poly p k = gsub p (k *! params_n) params_n
 
-unfold inline_for_extraction noextract
+inline_for_extraction noextract
 val index_poly: p: poly_k -> k: size_t{k <. params_k} -> Stack poly
     (requires fun h -> live h p)
-    (ensures  fun h0 r h1 -> h0 == h1 /\ live h1 r /\ r == gsub p (k *. params_n) params_n /\
+    (ensures  fun h0 r h1 -> h0 == h1 /\ live h1 r /\ r == gsub p (k *! params_n) params_n /\
                           loc_includes (loc p) (loc r))
-let index_poly p k = sub p (k *. params_n) params_n
+let index_poly p k = sub p (k *! params_n) params_n
 
 val reduce:
     a: I64.t{let q = elem_v params_q in let va = I64.v a in va <= (q-1)*(q-1)}
@@ -262,23 +239,27 @@ let shift_arithmetic_left x s =
     //Int.shift_left_value_lemma (I32.v x) (UI32.v s);
     //assert(I32.v r == I32.v x * pow2 (UI32.v s));
     //r
-(* {:pattern bget h1 s i}*) 
-let lemma_is_s_still_sk (h0 h1: HS.mem) (s: lbuffer sparse_elem params_n) : Lemma (ensures True) = ()
-//    (requires is_s_sk h0 s /\ 
-//              (forall (i:nat{i < v params_n}) . bget h0 s i == bget h1 s i))
-//    (ensures is_s_sk h0 s) = ()
-    //assert(forall (i:nat{i < v params_n}) . {:pattern is_sparse_elem_sk (bget h0 s i)} is_sparse_elem_sk (bget h0 s i))
-    //assert((is_s_sk h0 s) ==> (forall (i:nat{i < v params_n}) . is_sparse_elem_sk (bget h0 s i)));
-    //assert(is_s_sk h0 s);
-    //assert(forall (i:nat{i < v params_n}) . {:pattern is_sparse_elem_sk (bget h0 s i)} is_sparse_elem_sk (bget h0 s i));
-    //assert(forall (i:nat{i < v params_n}) . {:pattern bget h1 s i} bget h0 s i == bget h1 s i);
 
-let lemma_is_e_still_sk (h0 h1: HS.mem) (e: lbuffer sparse_elem (params_n *. params_k)) : Lemma (ensures True) = ()
-//    (requires is_e_sk h0 e /\ 
-//              (forall (i:nat{i < v params_n * v params_k}) . {:pattern bget h1 e i} bget h0 e i == bget h1 e i))
-//    (ensures is_e_sk h0 e) = ()
-    //assert(is_s_sk h0 s);
-    //assert(forall (i:nat{i < v params_n}) . {:pattern is_sparse_elem_sk (bget h0 s i)} is_sparse_elem_sk (bget h0 s i));
-    //assert(forall (i:nat{i < v params_n}) . {:pattern bget h1 s i} bget h0 s i == bget h1 s i);
-    //admit()
+(*let frame_is_poly_sampler_output_i (h0 h1: HS.mem) (p: poly) (i:nat{i <= v params_n}) (l:B.loc) : Lemma
+    (requires is_poly_sampler_output_i h0 p i /\ modifies l h0 h1 /\ disjoint l (gsub p (size 0) (size i)))
+    (ensures is_poly_sampler_output_i h1 p i)
+    [SMTPat (is_poly_sampler_output_i h1 p i); SMTPat (modifies l h0 h1)] =
+    assert(is_poly_equal h0 h1 p)*)
 
+(*let frame_is_poly_sampler_output_i (h0 h1: HS.mem) (p: B.lbuffer elem (v params_n)) (i:nat{i <= v params_n}) (l:B.loc) : Lemma
+    (requires is_poly_sampler_output_i h0 p i /\ B.modifies l h0 h1 /\ B.loc_disjoint l (B.loc_buffer p)) //(B.loc_buffer (B.gsub p 0ul (UI32.uint_to_t i))))
+    (ensures is_poly_sampler_output_i h1 p i)
+    [SMTPat (is_poly_sampler_output_i h1 p i); SMTPat (B.modifies l h0 h1)] = 
+    assert(forall (j:nat{j < i}) . {:pattern B.get h1 p j} B.get h0 p j == B.get h1 p j)*)
+
+(*let frame_is_poly_sampler_output_i (h0 h1: HS.mem) (p: poly) (i:nat{i <= v params_n}) (l:B.loc) : Lemma
+    (requires is_poly_sampler_output_i h0 p i /\ B.modifies l h0 h1 /\ B.loc_disjoint l (loc ((gsub p (size 0) (size i)))))
+    (ensures is_poly_sampler_output_i h1 p i)
+    [SMTPat (is_poly_sampler_output_i h1 p i); SMTPat (modifies l h0 h1)] = admit()
+    //assert(forall (j:nat{j < i}) . {:pattern bget h1 p j} bget h0 p j == bget h1 p j)
+    //assert(is_poly_equal h0 h1 p)*)
+
+(*let frame_is_poly_sampler_output_i (h0 h1: HS.mem) (p:poly) (i:nat{i <= v params_n}) (l:B.loc) : Lemma
+    (requires is_poly_sampler_output_i h0 p i /\ B.modifies l h0 h1 /\ B.loc_disjoint l (loc p))
+    (ensures is_poly_sampler_output_i h1 p i) = 
+    assert(forall (j:nat{j < i}) . {:pattern bget h1 p j} bget h0 p j == bget h1 p j)*)
